theories/FOL/Reification/PA_reflection.v
@@ -2,111 +2,16 @@ Require Import Undecidability.FOL.Util.Syntax.
 Require Import Undecidability.FOL.Util.FullTarski.
 Require Import Undecidability.FOL.Util.FullDeduction.
 Require Import Undecidability.FOL.Reification.GeneralReflection.
+Require Import Undecidability.FOL.PA.
+Import MetaCoq.Template.Ast MetaCoq.Template.TemplateMonad.Core.
 Import Vector.VectorNotations.
 Require Import String List.
 
 (* ** Signature for PA axiomatisation, containing function symbols for set operations *)
 
-Existing Instance falsity_on.
 
-
-Inductive PA_funcs : Type :=
-  Zero : PA_funcs
-| Succ : PA_funcs
-| Plus : PA_funcs
-| Mult : PA_funcs.
-
-Definition PA_funcs_ar (f : PA_funcs ) :=
-match f with
- | Zero => 0
- | Succ => 1
- | Plus => 2
- | Mult => 2
- end.
-
-Inductive PA_preds : Type :=
-  Eq : PA_preds.
-
-Definition PA_preds_ar (P : PA_preds) :=
-match P with
- | Eq => 2
-end.
-
-
-Instance PA_funcs_signature : funcs_signature :=
-{| syms := PA_funcs ; ar_syms := PA_funcs_ar |}.
-
-Instance PA_preds_signature : preds_signature :=
-{| preds := PA_preds ; ar_preds := PA_preds_ar |}.
-
-
-
-
-Declare Scope PA_Notation.
-Open Scope PA_Notation.
-
-Notation "'zero'" := (@func _ Zero ([])) (at level 1) : PA_Notation.
-Notation "'σ' x" := (@func _ Succ ([x])) (at level 37) : PA_Notation.
-Notation "x '⊕' y" := (@func _ Plus ([x ; y]) ) (at level 39) : PA_Notation.
-Notation "x '⊗' y" := (@func _ Mult ([x ; y]) ) (at level 38) : PA_Notation.
-Notation "x '==' y" := (@atom _ _ _ _ Eq ([x ; y])) (at level 40) : PA_Notation.
-Notation "x '⧀' y"  := (∃ (x[↑] ⊕ σ $0) == y) (at level 42) : PA_Notation.
 
 Fixpoint num n := match n with 0 => zero | S n => σ (num n) end.
-
-(* ** Axioms of PA *)
-
-
-Definition ax_zero_succ := ∀  (zero == σ var 0 ~> falsity).
-Definition ax_succ_inj :=  ∀∀ (σ $1 == σ $0 ~> $1 == $0).
-Definition ax_add_zero :=  ∀  (zero ⊕ $0 == $0).
-Definition ax_add_rec :=   ∀∀ ((σ $0) ⊕ $1 == σ ($0 ⊕ $1)).
-Definition ax_mult_zero := ∀  (zero ⊗ $0 == zero).
-Definition ax_mult_rec :=  ∀∀ (σ $1 ⊗ $0 == $0 ⊕ $1 ⊗ $0).
-
-Definition ax_induction (phi : form) :=
-  phi[zero..] ~> (∀ phi ~> phi[σ $0 .: S >> var]) ~> ∀ phi.
-
-
-
-(* Fragment only containing the defining equations for addition and multiplication. *)
-Definition FA := ax_add_zero :: ax_add_rec :: ax_mult_zero :: ax_mult_rec :: nil.
-
-(* Full axiomatisation of the theory of PA *)
-Inductive PA : form -> Prop :=
-  PA_FA phi : In phi FA -> PA phi
-| PA_discr : PA ax_zero_succ
-| PA_inj : PA ax_succ_inj
-| PA_induction phi : PA (ax_induction phi).
-
-
-
-(* Equality axioms for the PA signature *)
-
-Definition ax_refl :=  ∀   $0 == $0.
-Definition ax_sym :=   ∀∀  $1 == $0 ~> $0 == $1.
-Definition ax_trans := ∀∀∀ $2 == $1 ~> $1 == $0 ~> $2 == $0.
-
-Definition ax_succ_congr := ∀∀ $0 == $1 ~> σ $0 == σ $1.
-Definition ax_add_congr := ∀∀∀∀ $0 == $1 ~> $2 == $3 ~> $0 ⊕ $2 == $1 ⊕ $3.
-Definition ax_mult_congr := ∀∀∀∀ $0 == $1 ~> $2 == $3 ~> $0 ⊗ $2 == $1 ⊗ $3.
-
-
-Definition EQ :=
-  ax_refl :: ax_sym :: ax_trans :: ax_succ_congr :: ax_add_congr :: ax_mult_congr :: nil.
-
-Definition FAeq :=
-  EQ ++ FA.
-
-Inductive PAeq : form -> Prop :=
-  PAeq_FA phi : In phi FAeq -> PAeq phi
-| PAeq_discr : PAeq ax_zero_succ
-| PAeq_inj : PAeq ax_succ_inj
-| PAeq_induction phi : PAeq (ax_induction phi).
-
-Notation extensional M :=
-  (forall x y, @i_atom _ _ _ M Eq ([x ; y]) <-> x = y).
-
 
 Section ReificationExample.
   Context (D':Type).
@@ -117,64 +22,24 @@ Section ReificationExample.
   Notation "'iσ' x" := (@i_func _ _ D' I Succ ([x])) (at level 37) : PA_Notation.
   Notation "x 'i⊕' y" := (@i_func _ _ D' I Plus ([x ; y]) ) (at level 39) : PA_Notation.
   Notation "x 'i⊗' y" := (@i_func _ _ D' I Mult ([x ; y]) ) (at level 38) : PA_Notation.
+  Notation "x 'i=' y" := (@i_atom _ _ D' I Eq ([x ; y]) ) (at level 40) : PA_Notation.
+  Open Scope string_scope.
 
   Fixpoint inum n := match n with 0 => izero | S n => iσ (inum n) end.
+  Definition proj1 {X:Type} {Y:X->Type} (H:{x:X&Y x}) : X := match H with existT x y => x end.
+  Definition proj2 {X:Type} {Y:X->Type} (H:{x:X&Y x}) : Y (proj1 H) := match H with existT x y => y end.
 
-
-  Open Scope string_scope.
   Instance PA_reflector : tarski_reflector := buildDefaultTarski 
                         (i_func (f:=Zero) (Vector.nil D')) 
-                        (fun k => match k with (Ast.tVar "D'") => true | _ => false end).
+                        (anyVariableOf ("D'" :: nil)).
 
-  Section ReflectionExtension.
-    Import MetaCoq.Template.Ast MetaCoq.Template.TemplateMonad.Core.
-    Definition mergeNum (rho:nat -> D) (n:nat) : representsF (inum n) (num n) rho.
-    Proof. unfold representsF. induction n.
-    * easy.
-    * cbn. do 2 f_equal. cbn in IHn. now rewrite IHn.
-    Defined.
-    MetaCoq Quote Definition qNum := inum.
-    MetaCoq Quote Definition qMergeNum := mergeNum.
-    MetaCoq Quote Definition qMergeTermNum := @num.
+  Lemma example (a b : D) : representableP 0 (a i⊕ b i= b i⊕ a).
+  Proof. represent. Show Proof. Defined. (* Defined, so we can pull out the representative witness later *)
 
-    Definition mergeEqProp (rho:nat -> D) (d1 d2 : D) (t1 t2 : Syntax.term) : representsF d1 t1 rho -> representsF d2 t2 rho -> @representsP _ _ 0 (t1==t2) rho (d1 = d2).
-    Proof. intros pt1 pt2. cbn. unfold representsF in pt1, pt2. cbn in pt1, pt2. rewrite pt1, pt2. now rewrite D_ext.
-    Defined.
-    Definition mEq := (constructForm Eq).
-    MetaCoq Quote Definition qMergeFormEq := @mEq.
-    MetaCoq Quote Definition qMergeEqProp := mergeEqProp.
-    Definition reifyCoqEq : baseConnectiveReifier := fun tct qff l fuel envTerm env fPR fTR => match l with (tv::x::y::nil) => if maybeD tct tv then
-                                               xr <- fTR tct qff x envTerm env ;;
-                                               yr <- fTR tct qff y envTerm env ;; let '((xt,xp),(yt,yp)) := (xr,yr) in
-                                               ret (tApp qMergeFormEq (xt::yt::nil), tApp qMergeEqProp (envTerm::x::y::xt::yt::xp::yp::nil)) else fail "Eq applied to wrong type" | _ => fail "Eq constructor applied to != 2 terms" end.
-    Definition varsCoqEq : baseConnectiveVars := fun lst fuel tct _ fUVT => match lst with tv::x::y::nil => if maybeD tct tv then
-                                               xr <- fUVT x;;
-                                               yr <- fUVT y;;
-                                               ret (List.app xr yr) else fail "Eq applied to wrong type" | _ => fail "Eq constructor applied to != 2 terms" end.
-    Definition reifyBLC (s:string) : baseConnectiveReifier := match s with "eq" => reifyCoqEq | _ => fun _ _ _ _ _ _ _ _ => fail ("Unknown connective " ++ s) end.
-    Definition varsBLC (s:string) : baseConnectiveVars := match s with "eq" => varsCoqEq | _ => fun _ _ _ _ _ => fail ("Unknown connective " ++ s) end.
-    Definition findVarsTerm : termFinderVars := fun fuel t fUVT => match t with (tApp qMu (k::nil)) => ret nil | _ => fail "Fail" end.
-    Definition reifyTerm : termFinderReifier := fun tct qff fuel t envTerm env fTR => match t with tApp qMu (k::nil) => ret (tApp qMergeTermNum (k::nil), tApp qMergeNum (envTerm::k::nil)) | _ => fail "Fail" end.
-  End ReflectionExtension.
-  Instance PA_reflector_ext : tarski_reflector_extensions PA_reflector := {| (*Cannot define instance in section because they are dropped afterwards *)
-    baseLogicConnHelper := Some (reifyBLC);
-    baseLogicVarHelper := Some (varsBLC);
-    termReifierVarHelper := Some (findVarsTerm);
-    termReifierReifyHelper := Some (reifyTerm);
-    formReifierVarHelper := None;
-    formReifierReifyHelper := None
-  |}.
+  Eval cbn in (proj1 (example izero izero)).
 
-  MetaCoq Quote Definition tct := PA_reflector.
-  Definition proj1 {X:Type} {Y:X->Type} (H:{x:X&Y x}) : X := match H with existT x y => x end.
 
-  Lemma foo (a : D) (n:nat) : representableP 1 (fun (b:D) => forall (c:D), exists (d:D), a i⊕ b i⊗ c = iσ d /\ (True \/ ~False) <-> (inum n = inum n)).
-  Proof. represent.
-  Defined.
-
-  Eval cbn in (fun d n => proj1 (foo d n)).
-
-  Lemma bar : representableP 0 (~(True <-> False)).
+  Lemma only_logic : representableP 0 (~(True <-> False)).
   Proof. represent. Defined.
 
   Lemma large : representableP 0 
@@ -185,6 +50,54 @@ Section ReificationExample.
     /\ True /\ True /\ True \/ False /\ True /\ True /\ True \/ False /\ ~False \/ True <-> True
     \/ True /\ True /\ True \/ False /\ True /\ True /\ True \/ False /\ ~False \/ True <-> True).
   Proof. Time representNP. Restart. Time represent. Defined. 
+
+  Section ReflectionExtension.
+    (* Do a correctness proof for the specific extension *)
+    Definition mergeNum (rho:nat -> D) (n:nat) : representsF (inum n) (num n) rho.
+    Proof. unfold representsF. induction n.
+    * easy.
+    * cbn. do 2 f_equal. cbn in IHn. now rewrite IHn.
+    Defined.
+    (* Define some MetaCoq terms we will need later *)
+    MetaCoq Quote Definition qNum := inum.
+    MetaCoq Quote Definition qMergeNum := mergeNum.
+    MetaCoq Quote Definition qMergeTermNum := @num.
+
+    Definition mergeEqProp (rho:nat -> D) (d1 d2 : D) (t1 t2 : Syntax.term) : representsF d1 t1 rho -> representsF d2 t2 rho -> @representsP _ _ 0 (t1==t2) rho (d1 = d2).
+    Proof. intros pt1 pt2. cbn. unfold representsF in pt1, pt2. cbn in pt1, pt2. rewrite pt1, pt2. now rewrite D_ext.
+    Defined.
+    MetaCoq Quote Definition qMergeFormEq := (constructForm Eq).
+    MetaCoq Quote Definition qMergeEqProp := mergeEqProp.
+
+
+    Definition reifyCoqEq : baseConnectiveReifier := fun tct qff l fuel envTerm env fPR fTR => match l with (tv::x::y::nil) => if maybeD tct tv then
+                                               xr <- fTR tct qff x envTerm env ;;
+                                               yr <- fTR tct qff y envTerm env ;; let '((xt,xp),(yt,yp)) := (xr,yr) in
+                                               ret (tApp qMergeFormEq (xt::yt::nil), tApp qMergeEqProp (envTerm::x::y::xt::yt::xp::yp::nil)) else fail "Eq applied to wrong type" | _ => fail "Eq constructor applied to != 2 terms" end.
+    Definition varsCoqEq : baseConnectiveVars := fun lst fuel tct _ fUVT => match lst with tv::x::y::nil => if maybeD tct tv then
+                                               xr <- fUVT x;;
+                                               yr <- fUVT y;;
+                                               ret (List.app xr yr) else fail "Eq applied to wrong type" | _ => fail "Eq constructor applied to != 2 terms" end.
+    Definition reifyBLC (s:string) : baseConnectiveReifier := match s with "eq"%string => reifyCoqEq | _ => fun _ _ _ _ _ _ _ _ => fail ("Unknown connective " ++ s) end.
+    Definition varsBLC (s:string) : baseConnectiveVars := match s with "eq"%string => varsCoqEq | _ => fun _ _ _ _ _ => fail ("Unknown connective " ++ s) end.
+    Definition findVarsTerm : termFinderVars := fun fuel t fUVT => match t with (tApp qMu (k::nil)) => ret nil | _ => fail "Fail" end.
+    Definition reifyTerm : termFinderReifier := fun tct qff fuel t envTerm env fTR => match t with tApp qMu (k::nil) => ret (tApp qMergeTermNum (k::nil), tApp qMergeNum (envTerm::k::nil)) | _ => fail "Fail" end.
+  End ReflectionExtension.
+  (* If we want to extend the capabilities, we define an extension point instance *)
+  Instance PA_reflector_ext : tarski_reflector_extensions PA_reflector := {| (*Cannot define instance in section because they are dropped afterwards *)
+    baseLogicConnHelper := Some (reifyBLC);
+    baseLogicVarHelper := Some (varsBLC);
+    termReifierVarHelper := Some (findVarsTerm);
+    termReifierReifyHelper := Some (reifyTerm);
+    formReifierVarHelper := None;
+    formReifierReifyHelper := None
+  |}.
+
+  Lemma foo (a : D) (n:nat) : representableP 1 (fun (b:D) => forall (c:D), exists (d:D), a i⊕ b i⊗ c = iσ d /\ (True \/ ~False) <-> (inum n = inum n)).
+  Proof. represent. Defined.
+
+  Eval cbn in (fun d n => proj1 (foo d n)).
+
 
 
 End ReificationExample.
